Finished lazy evaluation

Evaluate.thy
@@ -5,163 +5,151 @@ begin
 inductive evaluate :: "expr \<Rightarrow> expr \<Rightarrow> bool" (infix "\<leadsto>" 60) where
   ev_app1 [simp]: "e\<^sub>1 \<leadsto> e\<^sub>1' \<Longrightarrow> App e\<^sub>1 e\<^sub>2 \<leadsto> App e\<^sub>1' e\<^sub>2" 
 | ev_app2 [simp]: "App (Abs t e\<^sub>1) e\<^sub>2 \<leadsto> Let e\<^sub>2 e\<^sub>1"
+| ev_app_let [simp]: "is_value e\<^sub>1\<^sub>2 \<Longrightarrow> App (Let e\<^sub>1\<^sub>1 e\<^sub>1\<^sub>2) e\<^sub>2 \<leadsto> Let e\<^sub>1\<^sub>1 (App e\<^sub>1\<^sub>2 (incr\<^sub>e\<^sub>e 0 e\<^sub>2))"
 | ev_let1 [simp]: "e\<^sub>2 \<leadsto> e\<^sub>2' \<Longrightarrow> Let e\<^sub>1 e\<^sub>2 \<leadsto> Let e\<^sub>1 e\<^sub>2'"
+| ev_let2 [simp]: "e\<^sub>1 \<leadsto> e\<^sub>1' \<Longrightarrow> head_var e\<^sub>2 = Some 0 \<Longrightarrow> Let e\<^sub>1 e\<^sub>2 \<leadsto> Let e\<^sub>1' e\<^sub>2"
+| ev_let3 [simp]: "is_value e\<^sub>1 \<Longrightarrow> head_var e\<^sub>2 = Some 0 \<Longrightarrow> Let e\<^sub>1 e\<^sub>2 \<leadsto> subst\<^sub>e\<^sub>e 0 e\<^sub>1 e\<^sub>2"
 | ev_rec [simp]: "list_all is_var vs \<Longrightarrow> \<not> is_var e \<Longrightarrow> 
     Rec (vs @ [e] @ nvs) \<leadsto> Let e (Rec (map (incr\<^sub>e\<^sub>e 0) vs @ [Var 0] @ map (incr\<^sub>e\<^sub>e 0) nvs))" 
 | ev_proj1 [simp]: "e \<leadsto> e' \<Longrightarrow> Proj e l \<leadsto> Proj e' l"
 | ev_proj2 [simp]: "list_all is_var fs \<Longrightarrow> lookup l fs = Some e \<Longrightarrow> Proj (Rec fs) l \<leadsto> e" 
+| ev_proj_let [simp]: "is_value e\<^sub>2 \<Longrightarrow> Proj (Let e\<^sub>1 e\<^sub>2) l \<leadsto> Let e\<^sub>1 (Proj e\<^sub>2 l)" 
 | ev_inj [simp]: "\<not> is_var e \<Longrightarrow> Inj l ts e \<leadsto> Let e (Inj l ts (Var 0))"
 | ev_case1 [simp]: "e \<leadsto> e' \<Longrightarrow> Case e t cs \<leadsto> Case e' t cs"
 | ev_case2 [simp]: "is_var e \<Longrightarrow> lookup l cs = Some e' \<Longrightarrow> Case (Inj l ts e) t cs \<leadsto> subst\<^sub>e\<^sub>e 0 e e'"
+| ev_case_let [simp]: "is_value e\<^sub>2 \<Longrightarrow> 
+    Case (Let e\<^sub>1 e\<^sub>2) t cs \<leadsto> Let e\<^sub>1 (Case e\<^sub>2 t (map (incr\<^sub>e\<^sub>e (Suc 0)) cs))" 
 | ev_fold [simp]: "\<not> is_var e \<Longrightarrow> Fold t e \<leadsto> Let e (Fold t (Var 0))" 
 | ev_unfold1 [simp]: "e \<leadsto> e' \<Longrightarrow> Unfold t e \<leadsto> Unfold t e'"  
 | ev_unfold2 [simp]: "is_var e \<Longrightarrow> Unfold t (Fold t e) \<leadsto> e" 
+| ev_unfold_let [simp]: "is_value e\<^sub>2 \<Longrightarrow> Unfold t (Let e\<^sub>1 e\<^sub>2) \<leadsto> Let e\<^sub>1 (Unfold t e\<^sub>2)" 
 | ev_tyapp1 [simp]: "e \<leadsto> e' \<Longrightarrow> TyApp e t \<leadsto> TyApp e' t" 
 | ev_tyapp2 [simp]: "TyApp (TyAbs k e) t \<leadsto> subst\<^sub>t\<^sub>e 0 t e" 
+| ev_tyapp_let [simp]: "is_value e\<^sub>2 \<Longrightarrow> TyApp (Let e\<^sub>1 e\<^sub>2) t \<leadsto> Let e\<^sub>1 (TyApp e\<^sub>2 t)" 
 | ev_tylet [simp]: "TyLet t e \<leadsto> subst\<^sub>t\<^sub>e 0 t e" 
 
-lemma [elim]: "e \<leadsto> e' \<Longrightarrow> is_value e \<Longrightarrow> False"
-  by (induction e e' rule: evaluate.induct) simp_all
+lemma canonical_arrow [simp]: "\<Delta>,\<Gamma> \<turnstile> e : Arrow t\<^sub>1 t\<^sub>2 \<Longrightarrow> is_value e \<Longrightarrow> 
+    (\<exists>e'. e = Abs t\<^sub>1 e') \<or> (\<exists>e\<^sub>1 e\<^sub>2. e = Let e\<^sub>1 e\<^sub>2 \<and> is_value e\<^sub>2)"
+  by (induction \<Gamma> e "Arrow t\<^sub>1 t\<^sub>2" rule: typecheck_typecheck_fs_typecheck_cs.inducts(1)) simp_all
 
-lemma [elim]: "e \<leadsto> e' \<Longrightarrow> is_var e \<Longrightarrow> False"
-  by (induction e e' rule: evaluate.induct) simp_all
+lemma canonical_record [simp]: "\<Delta>,\<Gamma> \<turnstile> e : Record ts \<Longrightarrow> is_value e \<Longrightarrow> 
+    (\<exists>fs. e = Rec fs \<and> list_all is_var fs \<and> \<Delta>,\<Gamma> \<turnstile>\<^sub>f fs : ts) \<or> (\<exists>e\<^sub>1 e\<^sub>2. e = Let e\<^sub>1 e\<^sub>2 \<and> is_value e\<^sub>2)"
+  by (induction \<Gamma> e "Record ts" rule: typecheck_typecheck_fs_typecheck_cs.inducts(1)) simp_all
 
-lemma [elim]: "list_all is_var vs \<Longrightarrow> list_all is_var vs' \<Longrightarrow> \<not> is_var e \<Longrightarrow> \<not> is_var e' \<Longrightarrow>
-    vs @ [e] @ nvs = vs' @ [e'] @ nvs' \<Longrightarrow> vs = vs'"
-  proof (induction vs arbitrary: vs')
-  case Nil
-    thus ?case by (induction vs') simp_all
-  next case (Cons v vs)
-    thus ?case by (induction vs') simp_all
-  qed
+lemma canonical_variant [simp]: "\<Delta>,\<Gamma> \<turnstile> e : Variant ts \<Longrightarrow> is_value e \<Longrightarrow> 
+    (\<exists>l e'. e = Inj l ts e' \<and> is_var e' \<and> l < length ts) \<or> (\<exists>e\<^sub>1 e\<^sub>2. e = Let e\<^sub>1 e\<^sub>2 \<and> is_value e\<^sub>2)"
+  by (induction \<Gamma> e "Variant ts" rule: typecheck_typecheck_fs_typecheck_cs.inducts(1)) auto
 
-theorem determinacy [elim]: "e \<leadsto> e' \<Longrightarrow> e \<leadsto> e'' \<Longrightarrow> e' = e''"
-  proof (induction e e' arbitrary: e'' rule: evaluate.induct)
-  case (ev_app1 e\<^sub>1 e\<^sub>1' e\<^sub>2)
-    with ev_app1(3) show ?case
-      proof (induction "App e\<^sub>1 e\<^sub>2" e'' rule: evaluate.induct)
-      case ev_app2
-        hence False by auto
-        thus ?case by simp
-      qed simp_all
-  next case (ev_app2 t e\<^sub>1 e\<^sub>2)
-    thus ?case by (induction "App (Abs t e\<^sub>1) e\<^sub>2" e'' rule: evaluate.induct) auto
-  next case (ev_let1 e\<^sub>2 e\<^sub>2' e\<^sub>1)
-    with ev_let1(3) show ?case by (induction "Let e\<^sub>1 e\<^sub>2" e'' rule: evaluate.induct) simp_all
-  next case (ev_rec vs e nvs)
-    with ev_rec(3) show ?case
-      proof (induction "Rec (vs @ [e] @ nvs)" e'' rule: evaluate.induct)
-      case (ev_rec vs' e\<^sub>2 nvs')
-        hence "vs' = vs" by auto
-        with ev_rec show ?case by simp
-      qed
-  next case (ev_proj1 e e' l)
-    with ev_proj1(3) show ?case
-      proof (induction "Proj e l" e'' rule: evaluate.induct)
-      case ev_proj2
-        hence False by auto
-        thus ?case by simp
-      qed simp_all
-  next case (ev_proj2 fs l e)
-    with ev_proj2(3) show ?case
-      proof (induction "Proj (Rec fs) l" e'' rule: evaluate.induct)
-      case ev_proj1
-        hence False by auto
-        thus ?case by simp
-      qed simp_all
-  next case (ev_inj e l ts)
-    with ev_inj(2) show ?case by (induction "Inj l ts e" e'' rule: evaluate.induct) simp_all
-  next case (ev_case1 e e' t cs)
-    with ev_case1(3) show ?case
-      proof (induction "Case e t cs" e'' rule: evaluate.induct)
-      case ev_case2
-        hence False by auto
-        thus ?case by simp
-      qed simp_all
-  next case (ev_case2 e l cs e' ts t)
-    with ev_case2(3) show ?case
-      proof (induction "Case (Inj l ts e) t cs" e'' rule: evaluate.induct)
-      case ev_case1
-        hence False by auto
-        thus ?case by simp
-      qed simp_all
-  next case (ev_fold e t)
-    with ev_fold(2) show ?case by (induction "Fold t e" e'' rule: evaluate.induct) simp_all
-  next case (ev_unfold1 e e' t)
-    with ev_unfold1(3) show ?case
-      proof (induction "Unfold t e" e'' rule: evaluate.induct)
-      case ev_unfold2
-        hence False by auto
-        thus ?case by simp
-      qed simp_all
-  next case (ev_unfold2 e t)
-    with ev_unfold2(2) show ?case
-      proof (induction "Unfold t (Fold t e)" e'' rule: evaluate.induct)
-      case ev_unfold1
-        hence False by auto
-        thus ?case by simp
-      qed simp_all
-  next case (ev_tyapp1 e e' t)
-    with ev_tyapp1(3) show ?case
-      proof (induction "TyApp e t" e'' rule: evaluate.induct)
-      case ev_tyapp2
-        hence False by auto
-        thus ?case by simp
-      qed simp_all
-  next case (ev_tyapp2 k e t)
+lemma canonical_inductive [simp]: "\<Delta>,\<Gamma> \<turnstile> e : Inductive k t \<Longrightarrow> is_value e \<Longrightarrow> 
+    (\<exists>e'. e = Fold t e' \<and> is_var e') \<or> (\<exists>e\<^sub>1 e\<^sub>2. e = Let e\<^sub>1 e\<^sub>2 \<and> is_value e\<^sub>2)"
+  by (induction \<Gamma> e "Inductive k t" rule: typecheck_typecheck_fs_typecheck_cs.inducts(1)) auto
+
+lemma canonical_forall [simp]: "\<Delta>,\<Gamma> \<turnstile> e : Forall k t \<Longrightarrow> is_value e \<Longrightarrow> 
+    (\<exists>e'. e = TyAbs k e') \<or> (\<exists>e\<^sub>1 e\<^sub>2. e = Let e\<^sub>1 e\<^sub>2 \<and> is_value e\<^sub>2)"
+  by (induction \<Gamma> e "Forall k t" rule: typecheck_typecheck_fs_typecheck_cs.inducts(1)) auto
+
+lemma lookup_in_tc [simp]: "\<Delta>,\<Gamma> \<turnstile>\<^sub>f fs : ts \<Longrightarrow> lookup l ts = Some t \<Longrightarrow> \<exists>e. lookup l fs = Some e"
+  by (induction l fs arbitrary: ts rule: lookup.induct) auto
+
+lemma split_fields [simp]: "\<not> list_all is_var fs \<Longrightarrow> 
+    \<exists>vs e nvs. fs = vs @ [e] @ nvs \<and> list_all is_var vs \<and> \<not> is_var e"
+  proof (induction fs)
+  case (Cons f fs)
     thus ?case
-      proof (induction "TyApp (TyAbs k e) t" e'' rule: evaluate.induct)
-      case ev_tyapp1
-        hence False by auto
-        thus ?case by simp
-      qed simp_all
-  next case (ev_tylet t e)
-    thus ?case by (induction "TyLet t e" e'' rule: evaluate.induct) simp_all
-  qed
-
-theorem progress: "\<Delta>,[] \<turnstile> e : t \<Longrightarrow> is_value e \<or> (\<exists>e'. e \<leadsto> e')"
-    and "\<Delta>,[] \<turnstile>\<^sub>f fs : ts \<Longrightarrow> True"
-    and "\<Delta>,[] \<turnstile>\<^sub>c cs : ts \<rightarrow> t \<Longrightarrow> l < length ts \<Longrightarrow> \<exists>c. lookup l cs = Some c"
-  proof (induction \<Delta> "[] :: type list" e t and \<Delta> "[] :: type list" fs ts 
-               and \<Delta> "[] :: type list" cs ts t
-         rule: typecheck_typecheck_fs_typecheck_cs.inducts)
-  case (tc_app \<Delta> e\<^sub>1 t\<^sub>1 t\<^sub>2 e\<^sub>2)
-    thus ?case by simp
-  next case (tc_let \<Delta> e\<^sub>1 t\<^sub>1 e\<^sub>2 t\<^sub>2)
-    thus ?case by simp
-  next case (tc_rec \<Delta> fs ts)
-    thus ?case by simp
-  next case (tc_proj \<Delta> e ts l t)
-    thus ?case by simp
-  next case (tc_inj \<Delta> e t l ts)
-    thus ?case by simp
-  next case (tc_case \<Delta> e ts cs t)
-    thus ?case by simp
-  next case (tc_fold \<Delta> e k t)
-    thus ?case by simp
-  next case (tc_unfold \<Delta> e k t)
-    thus ?case by simp
-  next case (tc_tyapp \<Delta> e k t t')
-    thus ?case by simp
-  next case (tc_tylet \<Delta> t' e t)
-    moreover have "TyLet t' e \<leadsto> subst\<^sub>t\<^sub>e 0 t' e" by simp
-    ultimately show ?case by fastforce
-  next case (tcc_cons t' e t fs ts)
-    thus ?case by simp
+      proof (cases "is_var f")
+      case True
+        with Cons obtain vs e nvs where "fs = vs @ [e] @ nvs \<and> list_all is_var vs \<and> \<not> is_var e" 
+          by fastforce
+        with True have "f # fs = (f # vs) @ [e] @ nvs \<and> list_all is_var (f # vs) \<and> \<not> is_var e" 
+          by simp
+        thus ?thesis by blast
+      qed fastforce+
   qed simp_all
 
-lemma preservation: "e \<leadsto> e' \<Longrightarrow> \<Delta>,\<Gamma> \<turnstile> e : t \<Longrightarrow> \<Delta>,\<Gamma> \<turnstile> e' : t"
+lemma progress': "\<Delta>,\<Gamma> \<turnstile> e : t \<Longrightarrow> 
+  is_value e \<or> (\<exists>e'. e \<leadsto> e') \<or> (\<exists>x < length \<Gamma>. head_var e = Some x)"
+    and "\<Delta>,\<Gamma> \<turnstile>\<^sub>f fs : ts \<Longrightarrow> True"
+    and "\<Delta>,\<Gamma> \<turnstile>\<^sub>c cs : ts \<rightarrow> t \<Longrightarrow> l < length ts \<Longrightarrow> \<exists>c. lookup l cs = Some c"
+  proof (induction \<Delta> \<Gamma> e t and \<Delta> \<Gamma> fs ts and \<Delta> \<Gamma> cs ts t
+         arbitrary: and and l
+         rule: typecheck_typecheck_fs_typecheck_cs.inducts)
+  case tc_var
+    thus ?case by (metis lookup_less_than head_var.simps(1))
+  next case tc_app
+    thus ?case by (metis canonical_arrow ev_app1 ev_app2 ev_app_let head_var.simps(3))
+  next case (tc_let \<Delta> \<Gamma> e\<^sub>1 t\<^sub>1 e\<^sub>2 t\<^sub>2)
+    thus ?case
+      proof (cases "is_value e\<^sub>2")
+      case False note F = False
+        thus ?thesis
+          proof (cases "\<exists>e\<^sub>2'. e\<^sub>2 \<leadsto> e\<^sub>2'")
+          case False
+            with tc_let F obtain x where X: "x < Suc (length \<Gamma>) \<and> head_var e\<^sub>2 = Some x" by fastforce
+            thus ?thesis 
+              proof (cases x)
+              case 0
+                with X show ?thesis
+                  proof (cases "is_value e\<^sub>1")
+                  case False
+                    with tc_let X 0 ev_let2 show ?thesis by fastforce
+                  qed (metis ev_let3)
+              qed simp_all
+          qed (metis ev_let1)
+      qed simp_all
+  next case tc_rec
+    thus ?case by (metis ev_rec is_value.simps(5) split_fields)
+  next case tc_proj
+    thus ?case 
+      by (metis canonical_record ev_proj1 ev_proj2 ev_proj_let head_var.simps(6) lookup_in_tc)
+  next case tc_inj
+    thus ?case by (metis ev_inj is_value.simps(7))
+  next case tc_case
+    thus ?case by (metis canonical_variant ev_case1 ev_case2 ev_case_let head_var.simps(8))
+  next case tc_fold
+    thus ?case by (metis ev_fold is_value.simps(9))
+  next case tc_unfold
+    thus ?case by (metis canonical_inductive ev_unfold1 ev_unfold2 ev_unfold_let head_var.simps(10))
+  next case tc_tyapp
+    thus ?case by simp (metis canonical_forall ev_tyapp1 ev_tyapp2 ev_tyapp_let)
+  next case tc_tylet
+    thus ?case by (metis ev_tylet)
+  next case tcc_cons
+    thus ?case by (induction l) simp_all
+  qed simp_all
+
+theorem progress: "\<Delta>,[] \<turnstile> e : t \<Longrightarrow> is_value e \<or> (\<exists>e'. e \<leadsto> e')"
+  using progress' by fastforce
+
+lemma [elim]: "\<Delta>,\<Gamma> \<turnstile>\<^sub>f fs : ts \<Longrightarrow> lookup l fs = Some e \<Longrightarrow> lookup l ts = Some t \<Longrightarrow> \<Delta>,\<Gamma> \<turnstile> e : t" 
+  by (induction l fs arbitrary: ts rule: lookup.induct) auto
+
+lemma [elim]: "\<Delta>,\<Gamma> \<turnstile>\<^sub>c cs : ts \<rightarrow> t \<Longrightarrow> lookup l cs = Some e \<Longrightarrow> lookup l ts = Some t' \<Longrightarrow> 
+    \<Delta>,insert_at 0 t' \<Gamma> \<turnstile> e : t" 
+  by (induction l cs arbitrary: ts rule: lookup.induct) auto
+
+theorem preservation: "e \<leadsto> e' \<Longrightarrow> \<Delta>,\<Gamma> \<turnstile> e : t \<Longrightarrow> \<Delta>,\<Gamma> \<turnstile> e' : t"
   proof (induction e e' arbitrary: \<Delta> \<Gamma> t rule: evaluate.induct) 
   case (ev_rec vs e nvs)
     then obtain tvs tenvs where "t = Record (tvs @ tenvs) \<and> (\<Delta>,\<Gamma> \<turnstile>\<^sub>f vs : tvs) 
       \<and> (\<Delta>,\<Gamma> \<turnstile>\<^sub>f [e] @ nvs : tenvs)" by fastforce
     thus ?case by fastforce
   next case (ev_inj e l ts)
-    thus ?case by simp
-  next case ev_case2
-    thus ?case by simp
-  next case ev_tyapp2
-    thus ?case by simp
+    then obtain t\<^sub>1 where T: "(\<Delta>,\<Gamma> \<turnstile> e : t\<^sub>1) \<and> lookup l ts = Some t\<^sub>1 \<and> 
+      (\<forall>tt \<in> set ts. \<Delta> \<turnstile>\<^sub>k tt : Star) \<and> t = Variant ts" by fastforce
+    have "\<Delta>,insert_at 0 t\<^sub>1 \<Gamma> \<turnstile> Var 0 : t\<^sub>1" by simp
+    with T have "\<Delta>,insert_at 0 t\<^sub>1 \<Gamma> \<turnstile> Inj l ts (Var 0) : Variant ts" by (metis tc_inj)
+    with T show ?case by (metis tc_let)
+  next case (ev_case2 e l cs e' ts t')
+    then obtain tt where "(\<Delta>,\<Gamma> \<turnstile> e : tt) \<and> lookup l ts = Some tt \<and> 
+      (\<forall>tt \<in> set ts. \<Delta> \<turnstile>\<^sub>k tt : Star) \<and> (\<Delta>,\<Gamma> \<turnstile>\<^sub>c cs : ts \<rightarrow> t') \<and> t' = t" by fastforce
+    moreover with ev_case2 have "\<Delta>,insert_at 0 tt \<Gamma> \<turnstile> e' : t" by fastforce
+    ultimately show ?case by simp
+  next case (ev_tyapp2 k e t')
+    then obtain tt where T: "(insert_at 0 k \<Delta>,map (incr\<^sub>t\<^sub>t 0) \<Gamma> \<turnstile> e : tt) \<and> (\<Delta> \<turnstile>\<^sub>k t' : k) \<and> 
+      t = subst\<^sub>t\<^sub>t 0 t' tt" by fastforce
+    moreover hence "\<Delta>,map (subst\<^sub>t\<^sub>t 0 t') (map (incr\<^sub>t\<^sub>t 0) \<Gamma>) \<turnstile> subst\<^sub>t\<^sub>e 0 t' e : subst\<^sub>t\<^sub>t 0 t' tt" 
+      using tc_subst\<^sub>t\<^sub>e by fastforce
+    ultimately show ?case by simp
   qed fastforce+
 
 end
