Determinism.thy
@@ -1,0 +1,188 @@
+theory Determinism
+imports Evaluate
+begin
+
+lemma [elim]: "head_var e = Some x \<Longrightarrow> is_value e \<Longrightarrow> False"
+  by (induction e arbitrary: x) (auto split: option.splits nat.splits)
+
+lemma [elim]: "e \<leadsto> e' \<Longrightarrow> is_value e \<Longrightarrow> False"
+  by (induction e e' rule: evaluate.induct) auto
+
+lemma [elim]: "e \<leadsto> e' \<Longrightarrow> is_var e \<Longrightarrow> False"
+  by (induction e e' rule: evaluate.induct) simp_all
+
+lemma [elim]: "e \<leadsto> e' \<Longrightarrow> head_var e = Some x \<Longrightarrow> False"
+  by (induction e e' arbitrary: x rule: evaluate.induct) (auto split: option.splits nat.splits)
+
+lemma [elim]: "list_all is_var vs \<Longrightarrow> list_all is_var vs' \<Longrightarrow> \<not> is_var e \<Longrightarrow> \<not> is_var e' \<Longrightarrow>
+    vs @ [e] @ nvs = vs' @ [e'] @ nvs' \<Longrightarrow> vs = vs'"
+  proof (induction vs arbitrary: vs')
+  case Nil
+    thus ?case by (induction vs') simp_all
+  next case (Cons v vs)
+    thus ?case by (induction vs') simp_all
+  qed
+
+theorem determinism [elim]: "e \<leadsto> e' \<Longrightarrow> e \<leadsto> e'' \<Longrightarrow> e' = e''"
+  proof (induction e e' arbitrary: e'' rule: evaluate.induct)
+  case (ev_app1 e\<^sub>1 e\<^sub>1' e\<^sub>2)
+    with ev_app1(3) show ?case
+      proof (induction "App e\<^sub>1 e\<^sub>2" e'' rule: evaluate.induct)
+      case ev_app2
+        hence False by auto
+        thus ?case by simp
+      next case ev_app_let
+        hence False by auto
+        thus ?case by simp
+      qed simp_all
+  next case (ev_app2 t e\<^sub>1 e\<^sub>2)
+    thus ?case by (induction "App (Abs t e\<^sub>1) e\<^sub>2" e'' rule: evaluate.induct) auto
+  next case (ev_app_let e\<^sub>1\<^sub>2 e\<^sub>1\<^sub>1 e\<^sub>2)
+    with ev_app_let(2) show ?case
+      proof (induction "App (Let e\<^sub>1\<^sub>1 e\<^sub>1\<^sub>2) e\<^sub>2" e'' rule: evaluate.induct)
+      case ev_app1
+        hence False by auto
+        thus ?case by simp
+      qed simp_all
+  next case (ev_let1 e\<^sub>2 e\<^sub>2' e\<^sub>1)
+    with ev_let1(3) show ?case
+      proof (induction "Let e\<^sub>1 e\<^sub>2" e'' rule: evaluate.induct) 
+      case ev_let2
+        hence False by fast
+        thus ?case by simp
+      next case ev_let3
+        hence False by auto
+        thus ?case by simp
+      qed simp_all
+  next case (ev_let2 e\<^sub>1 e\<^sub>1' e\<^sub>2)
+    with ev_let2(4) show ?case
+      proof (induction "Let e\<^sub>1 e\<^sub>2" e'' rule: evaluate.induct) 
+      case ev_let1
+        hence False by fast
+        thus ?case by simp
+      next case ev_let3
+        hence False by auto
+        thus ?case by simp
+      qed simp_all
+  next case (ev_let3 e\<^sub>1 e\<^sub>2)
+    with ev_let3(3) show ?case
+      proof (induction "Let e\<^sub>1 e\<^sub>2" e'' rule: evaluate.induct) 
+      case ev_let1
+        hence False by auto
+        thus ?case by simp
+      next case ev_let2
+        hence False by auto
+        thus ?case by simp
+      qed simp_all
+  next case (ev_rec vs e nvs)
+    with ev_rec(3) show ?case
+      proof (induction "Rec (vs @ [e] @ nvs)" e'' rule: evaluate.induct)
+      case (ev_rec vs' e\<^sub>2 nvs')
+        hence "vs' = vs" by auto
+        with ev_rec show ?case by simp
+      qed
+  next case (ev_proj1 e e' l)
+    with ev_proj1(3) show ?case
+      proof (induction "Proj e l" e'' rule: evaluate.induct)
+      case ev_proj2
+        hence False by auto
+        thus ?case by simp
+      next case ev_proj_let
+        hence False by auto
+        thus ?case by simp
+      qed simp_all
+  next case (ev_proj2 fs l e)
+    with ev_proj2(3) show ?case
+      proof (induction "Proj (Rec fs) l" e'' rule: evaluate.induct)
+      case ev_proj1
+        hence False by auto
+        thus ?case by simp
+      qed simp_all
+  next case (ev_proj_let e\<^sub>2 e\<^sub>1 l)
+    with ev_proj_let(2) show ?case
+      proof (induction "Proj (expr.Let e\<^sub>1 e\<^sub>2) l" e'' rule: evaluate.induct)
+      case ev_proj1
+        hence False by auto
+        thus ?case by simp
+      qed simp_all
+  next case (ev_inj e l ts)
+    with ev_inj(2) show ?case by (induction "Inj l ts e" e'' rule: evaluate.induct) simp_all
+  next case (ev_case1 e e' t cs)
+    with ev_case1(3) show ?case
+      proof (induction "Case e t cs" e'' rule: evaluate.induct)
+      case ev_case2
+        hence False by auto
+        thus ?case by simp
+      next case ev_case_let
+        hence False by auto
+        thus ?case by simp
+      qed simp_all
+  next case (ev_case2 e l cs e' ts t)
+    with ev_case2(3) show ?case
+      proof (induction "Case (Inj l ts e) t cs" e'' rule: evaluate.induct)
+      case ev_case1
+        hence False by auto
+        thus ?case by simp
+      qed simp_all
+  next case (ev_case_let e\<^sub>2 e\<^sub>1 t cs)
+    with ev_case_let(2) show ?case
+      proof (induction "Case (Let e\<^sub>1 e\<^sub>2) t cs" e'' rule: evaluate.induct)
+      case ev_case1
+        hence False by auto
+        thus ?case by simp
+      qed simp_all
+  next case (ev_fold e t)
+    with ev_fold(2) show ?case by (induction "Fold t e" e'' rule: evaluate.induct) simp_all
+  next case (ev_unfold1 e e' t)
+    with ev_unfold1(3) show ?case
+      proof (induction "Unfold t e" e'' rule: evaluate.induct)
+      case ev_unfold2
+        hence False by auto
+        thus ?case by simp
+      next case ev_unfold_let
+        hence False by auto
+        thus ?case by simp
+      qed simp_all
+  next case (ev_unfold2 e t)
+    with ev_unfold2(2) show ?case
+      proof (induction "Unfold t (Fold t e)" e'' rule: evaluate.induct)
+      case ev_unfold1
+        hence False by auto
+        thus ?case by simp
+      qed simp_all
+  next case (ev_unfold_let e\<^sub>2 e\<^sub>1 t)
+    with ev_unfold_let(2) show ?case
+      proof (induction "Unfold e\<^sub>1 (Let t e\<^sub>2)" e'' rule: evaluate.induct)
+      case ev_unfold1
+        hence False by auto
+        thus ?case by simp
+      qed simp_all
+  next case (ev_tyapp1 e e' t)
+    with ev_tyapp1(3) show ?case
+      proof (induction "TyApp e t" e'' rule: evaluate.induct)
+      case ev_tyapp2
+        hence False by auto
+        thus ?case by simp
+      next case ev_tyapp_let
+        hence False by auto
+        thus ?case by simp
+      qed simp_all
+  next case (ev_tyapp2 k e t)
+    thus ?case
+      proof (induction "TyApp (TyAbs k e) t" e'' rule: evaluate.induct)
+      case ev_tyapp1
+        hence False by auto
+        thus ?case by simp
+      qed simp_all
+  next case (ev_tyapp_let e\<^sub>2 e\<^sub>1 t)
+    with ev_tyapp_let(2) show ?case
+      proof (induction "TyApp (Let e\<^sub>1 e\<^sub>2) t" e'' rule: evaluate.induct)
+      case ev_tyapp1
+        hence False by auto
+        thus ?case by simp
+      qed simp_all
+  next case (ev_tylet t e)
+    thus ?case by (induction "TyLet t e" e'' rule: evaluate.induct) simp_all
+  qed
+
+end
